attribute_list_length spec and verification proof

verif/db/verif_operations.v
@@ -1,7 +1,4 @@
 Require Import VST.floyd.proofauto.
-Require Import VST.msl.iter_sepcon.
-Require Import VST.floyd.reassoc_seq.
-Require Import VST.floyd.field_at_wand.
 
 Require Import Signatures.
 
@@ -59,24 +56,59 @@ Definition attribute_string_rep sh (a : attribute) (p : val) : mpred :=
 
 Fixpoint attribute_lseg_rep (sh : share) (l : list attribute) (p q : val) : mpred :=
   match l with
-  | [] => !! (p = q) && emp
+  | [] => !! (p = q /\ is_pointer_or_null p) && emp
   | a :: tl =>
     EX r : val, EX sptr : val, data_at sh t_attr_list (sptr, (domain_of_attribute a, r)) p * attribute_lseg_rep sh tl r q * attribute_string_rep sh a sptr end.
 
+Lemma attribute_lseg_nil sh l : attribute_lseg_rep sh l nullval nullval |-- !! (l = []).
+Proof.
+  destruct l; simpl; entailer.
+  saturate_local. apply field_compatible_nullval with (P := False) in H.
+  contradiction.
+Qed.
+ 
 Definition attribute_list_rep sh l p := attribute_lseg_rep sh l p nullval.
 
-Lemma attribute_list_rep_valid_pointer:
+Lemma attribute_lseg_rep_local_facts:
+  forall sh l p q,
+   attribute_lseg_rep sh l p q |--
+                      !! (is_pointer_or_null p /\ is_pointer_or_null q).
+Proof.
+  induction l; intros; unfold attribute_lseg_rep; entailer.
+  fold attribute_lseg_rep. sep_apply IHl. entailer.
+Qed.
+
+Hint Resolve attribute_lseg_rep_local_facts : saturate_local.
+
+Lemma attribute_list_rep_local_facts:
   forall sh l p,
+   attribute_list_rep sh l p |--
+                      !! (is_pointer_or_null p /\ (p=nullval <-> l=nil)).
+Proof.
+  unfold attribute_list_rep, attribute_lseg_rep. induction l; intros; entailer.
+  entailer!. easy.
+  fold attribute_lseg_rep in IHl |- *.
+  sep_apply (IHl r). entailer!. apply field_compatible_nullval1 in H0.
+  easy.
+Qed.
+
+Hint Resolve attribute_list_rep_local_facts : saturate_local.
+
+Lemma attribute_list_rep_valid_pointer:
+  forall sh l p, readable_share sh ->
    attribute_list_rep sh l p |-- valid_pointer p.
 Proof.
   intros.
-  unfold attribute_list_rep; destruct l; simpl; entailer!. Admitted.
+  unfold attribute_list_rep; destruct l; simpl. entailer.
+  Intros r sptr. sep_apply data_at_valid_ptr.
+  apply readable_nonidentity. assumption.
+  entailer.
+Qed.
 
 Hint Resolve attribute_list_rep_valid_pointer : valid_pointer.
 
 Definition attributes_rep (sh : share) (attrs : Fset.set FAN) (p : val) : mpred :=
-  let attrs_list := Fset.elements _ attrs in
-  attribute_list_rep sh attrs_list p.
+  attribute_list_rep sh ({{{attrs}}}) p.
 
 Definition attribute_list_length_spec :=
  DECLARE _attribute_list_length
@@ -91,18 +123,34 @@ Definition attribute_list_length_spec :=
      SEP (attributes_rep sh attrs l).
 
 Definition Gprog := ltac:(with_library prog [attribute_list_length_spec]).
-
-Lemma body_sumarray: semax_body Vprog Gprog f_attribute_list_length attribute_list_length_spec.
+Print Fset.
+Lemma body_attribute_list_length: semax_body Vprog Gprog f_attribute_list_length attribute_list_length_spec.
 Proof.
   start_function.
-  forward.
-  forward.
+  forward. forward.
   forward_loop
     (EX x : val, EX l1 : list attribute, EX l2 : list attribute,
-            PROP ( Fset.elements _ attrs = l1 ++ l2 )
+            PROP ( {{{attrs}}} = l1 ++ l2 )
                  LOCAL (temp _n (Vint (Int.repr (Zlength l1))); temp _x x; temp _l l)
-                 SEP (attribute_lseg_rep sh l1 l x * attribute_lseg_rep sh l2 x nullval )).
-  entailer. Exists l (@nil attribute) (Fset.elements _ attrs).
-  entailer!. simpl. unfold attributes_rep, attribute_list_rep. entailer.
-  entailer!.
-  
+                 SEP (attribute_lseg_rep sh l1 l x; attribute_list_rep sh l2 x ))%assert.
+  - Exists l (@nil attribute) (Fset.elements _ attrs).
+  entailer!. unfold attributes_rep, attribute_list_rep. simpl. entailer!.
+  - entailer!.
+  - destruct l2. unfold attribute_list_rep, attribute_lseg_rep at 2. 
+    Intros. rewrite H0 in HRE. contradiction.
+    unfold attribute_list_rep; unfold attribute_lseg_rep at 2; fold attribute_lseg_rep. 
+    Intros r sptr.
+    forward.
+    forward.
+    Exists (r, l1 ++ [a], l2). entailer!.
+    split. rewrite semax_lemmas.cons_app in H. rewrite app_assoc in H. auto.
+    rewrite Zlength_app. rewrite Zlength_cons. simpl. reflexivity.
+    unfold attribute_list_rep. cancel.
+    revert l PNl. generalize l1. induction l0; intros. rewrite app_nil_l. simpl. Exists r sptr. entailer.
+    simpl. Intros r0 sptr0. Exists r0 sptr0. entailer!.
+    apply IHl0. auto.
+  - forward. assert (h : l2 = []). rewrite <- H0; easy.
+    subst l2. rewrite app_nil_r in H. subst l1.
+    rewrite Fset.cardinal_spec. rewrite Zlength_correct; auto. entailer!.
+    unfold attributes_rep, attribute_list_rep. sep_apply attribute_lseg_nil. simpl. entailer!.
+Qed.
